WIP

examples/mw/MWApp1New.v
@@ -21,40 +21,106 @@ Section PROOF.
   Notation pget := (p0 <- trigger PGet;; p0 <- p0↓ǃ;; Ret p0) (only parsing).
   Notation pput p0 := (trigger (PPut p0↑)) (only parsing).
 
+  (* Definition ASSUME (P: iProp): itree Es unit := *)
+  (*   ri <- trigger (Take _);; *)
+  (*   assume(P ri);;; *)
+  (*   rm0 <- pget;; rm1 <- trigger (Take _);; assume(rm1 = rm0 ⋅ ri ∧ URA.wf rm1);;; pput rm1;;; *)
+  (*   Ret tt *)
+  (* . *)
+
+  (* Definition GUARANTEE (Q: iProp): itree Es unit := *)
+  (*   ro <- trigger (Choose _);; *)
+  (*   guarantee(Q ro);;; *)
+  (*   rm0 <- pget;; rm1 <- trigger (Choose _);; guarantee(rm1 ⋅ ro = rm0);;; *)
+  (*   Ret tt *)
+  (* . *)
+
+  (* Definition initF: list val -> itree Es val := *)
+  (*   fun varg => _ <- (pargs [] varg)?;; *)
+  (*     ASSUME(OwnM AppInit);;; *)
+
+  (*     GUARANTEE(⌜True⌝%I);;; *)
+  (*     `_: val <- ccallU "put" [Vint 0; Vint 42];; *)
+  (*     ASSUME(⌜True⌝%I);;; *)
+
+  (*     GUARANTEE(OwnM AppRun);;; *)
+
+  (*     Ret Vundef *)
+  (* . *)
+
+
+  (***
+     var ri := Take
+     assume(P ri)
+     rf := take(rf + rm + ri)
+   ***)
+
+  (***
+     var (rm, ro) := Choose
+     guarantee(Q ro)
+     rf := choose (rf - rm - ro)
+   ***)
+
+  Definition ASSUME rf0 (P: AppRA -> Prop): itree Es _ :=
+    ri <- trigger (Take _);;
+    assume(P ri);;;
+    rm <- pget;; rf1 <- trigger (Take _);; assume(rf1 = rm ⋅ ri ⋅ rf0 ∧ URA.wf rf1);;;
+    Ret rf1
+  .
+
+  Definition GUARANTEE rf0 (Q: AppRA -> Prop): itree Es _ :=
+    '(rm, ro, rf1) <- trigger (Choose _);;
+    guarantee(Q ro);;;
+    guarantee(rm ⋅ ro ⋅ rf1 = rf0);;; pput rm;;;
+    Ret rf1
+  .
+
   Definition initF: list val -> itree Es val :=
     fun varg => _ <- (pargs [] varg)?;;
-      ri <- trigger (Take _);;
-      assume(ri = AppInit);;;
-      rm0 <- pget;; rm1 <- trigger (Take _);; assume(rm1 = rm0 ⋅ rm1 ∧ URA.wf rm1);;; pput rm1;;;
+      let rf := ε in
+      rf <- (ASSUME rf (eq AppInit));;
 
+      rf <- (GUARANTEE rf top1);;
       `_: val <- ccallU "put" [Vint 0; Vint 42];;
+      rf <- (ASSUME rf top1);;
 
-      ro <- trigger (Choose _);;
-      guarantee(ro = AppRun);;;
-      rm2 <- pget;; rm3 <- trigger (Choose _);; guarantee(rm3 ⋅ ro = rm2);;;
+      rf <- (GUARANTEE rf (eq AppRun));;
 
       Ret Vundef
   .
 
+  (* Definition runF: list val -> itree Es val := *)
+  (*   fun varg => _ <- (pargs [] varg)?;; *)
+  (*     ri <- trigger (Take _);; *)
+  (*     assume(ri = AppInit);;; *)
+  (*     `rm0: AppRA <- pget;; rm1 <- trigger (Take _);; assume(rm1 = rm0 ⋅ ri ∧ URA.wf rm1);;; pput rm1;;; *)
+
+  (*     `v: val <- ccallU "get" [Vint 0];; trigger (Syscall "print" [v]↑ top1);;; *)
+
+  (*     ro <- trigger (Choose _);; *)
+  (*     guarantee(ro = AppRun);;; *)
+  (*     rm2 <- pget;; rm3 <- trigger (Choose _);; guarantee(rm3 ⋅ ro = rm2);;; *)
+
+  (*     Ret Vundef *)
+  (* . *)
+
   Definition runF: list val -> itree Es val :=
     fun varg => _ <- (pargs [] varg)?;;
-      ri <- trigger (Take _);;
-      assume(ri = AppInit);;;
-      rm0 <- pget;; rm1 <- trigger (Take _);; assume(rm1 = rm0 ⋅ rm1 ∧ URA.wf rm1);;; pput rm1;;;
+      let rf := ε in
+      rf <- (ASSUME rf (eq AppRun));;
 
+      rf <- (GUARANTEE rf top1);;
       `v: val <- ccallU "get" [Vint 0];; trigger (Syscall "print" [v]↑ top1);;;
+      rf <- (ASSUME rf top1);;
 
-      ro <- trigger (Choose _);;
-      guarantee(ro = AppRun);;;
-      rm2 <- pget;; rm3 <- trigger (Choose _);; guarantee(rm3 ⋅ ro = rm2);;;
-
+      rf <- GUARANTEE rf (eq AppRun);;
       Ret Vundef
   .
 
   Definition AppSem: ModSem.t := {|
     ModSem.fnsems := [("init", cfunU initF); ("run", cfunU runF)];
     ModSem.mn := "App";
-    ModSem.initial_st := (GRA.embed AppInitX)↑;
+    ModSem.initial_st := (AppInitX)↑;
   |}
   .
 
