examples/mw/MWApp01Newproof.v
@@ -1,0 +1,113 @@
+Require Import HoareDef MWHeader MWApp0 MWApp1New SimModSem.
+Require Import Coqlib.
+Require Import ImpPrelude.
+Require Import Skeleton.
+Require Import PCM.
+Require Import ModSem Behavior.
+Require Import Relation_Definitions.
+
+(*** TODO: export these in Coqlib or Universe ***)
+Require Import Relation_Operators.
+Require Import RelationPairs.
+From ITree Require Import
+     Events.MapDefault.
+From ExtLib Require Import
+     Core.RelDec
+     Structures.Maps
+     Data.Map.FMapAList.
+
+Require Import HTactics ProofMode.
+
+Set Implicit Arguments.
+
+Local Open Scope nat_scope.
+
+
+
+Section SIMMODSEM.
+
+  Context `{Σ: GRA.t}.
+  Context `{@GRA.inG AppRA Σ}.
+
+  Let W: Type := Any.t * Any.t.
+
+  Let wf: _ -> W -> Prop :=
+    (* @mk_wf *)
+    (*   _ *)
+    (*   unit *)
+    (*   (fun _ _ st_tgt => ((OwnM(AppInitX) ∧ ⌜st_tgt = false↑⌝) ∨ (OwnM(AppRunX) ∧ ⌜st_tgt = true↑⌝))%I) *)
+
+    fun (_: unit) '(mpr_src, mpr_tgt) => (mpr_src = (AppInitX)↑ ∧ mpr_tgt = false↑) ∨
+                                         (mpr_src = (AppRunX)↑ ∧ mpr_tgt = true↑)
+  .
+
+  Theorem correct: refines2 [MWApp0.App] [MWApp1New.App].
+  Proof.
+    eapply adequacy_local2. econs; ss.
+    i. econstructor 1 with (wf:=wf) (le:=top2); et; swap 2 3.
+    { ss. }
+    { esplits. econs; ss. }
+
+    econs; ss.
+    { init. steps. unfold initF, MWApp0.initF, ASSUME, GUARANTEE. steps.
+      rr in WF. des; clarify; rewrite Any.upcast_downcast in *; clarify.
+      2: { steps. des; clarify. admit "ez". }
+      steps. des; clarify. unfold ccallU. steps. force_l. exists (AppInitX, @URA.unit AppRA, AppInit).
+      steps. force_l; ss. steps. force_l; ss.
+      { admit "ez". }
+      steps. des; clarify; rewrite Any.upcast_downcast in *; clarify.
+      2: { steps. des; clarify. admit "ez". }
+      steps. force_l. exists (AppRunX, AppRun, @URA.unit AppRA). steps. force_l; ss. steps. des; clarify.
+      force_l; ss.
+      { admit "ez". }
+      steps. rr. esplits; et. rr. right; ss.
+    }
+    econs; ss.
+    { init. steps. unfold runF, MWApp0.runF, ASSUME, GUARANTEE. steps.
+      rr in WF. des; clarify; rewrite Any.upcast_downcast in *; clarify.
+      1: { steps. des; clarify. admit "ez". }
+      steps. des; clarify. unfold ccallU. steps. force_l. exists (AppRunX, @URA.unit AppRA, AppRun).
+      steps. force_l; ss. steps. force_l; ss.
+      { admit "ez". }
+      steps. des; clarify; rewrite Any.upcast_downcast in *; clarify.
+      1: { steps. des; clarify. admit "ez". }
+      steps. des; clarify. force_l. exists (AppRunX, AppRun, @URA.unit AppRA). steps. force_l; ss. steps.
+      force_l; ss.
+      { admit "ez". }
+      steps. rr. esplits; et. rr. right; ss.
+    }
+    (*   { left. ss. esplits; et. *)
+    (*   des; clarify. *)
+    (*   { rewrite Any.upcast_downcast in *. clarify. steps. *)
+    (*   harg. mDesAll. des; clarify. unfold initF, ccallU. steps. *)
+    (*   mDesOr "INV"; mDesAll; des; clarify. *)
+    (*   2: { mAssertPure False; ss. iCombine "INV A" as "A". iOwnWf "A" as WF0. admit "ez". } *)
+    (*   steps. rewrite Any.upcast_downcast in *. clarify. steps. *)
+    (*   hcall _ _ _ with "INV"; auto. *)
+    (*   { esplits; ss. } *)
+    (*   steps. mDesAll; clarify. mDesOr "INV1"; mDesAll; clarify. *)
+    (*   2: { mAssertPure False; ss. iCombine "INV1 A" as "A". iOwnWf "A" as WF0. admit "ez". } *)
+    (*   rewrite _UNWRAPU. steps. *)
+    (*   mAssert _ with "*". *)
+    (*   { iCombine "A" "INV1" as "A". iApply (OwnM_Upd with "A"). *)
+    (*     instantiate (1:=AppRun ⋅ AppRunX). admit "ez". } *)
+    (*   hret _; ss. *)
+    (*   { iMod "A1". iDestruct "A1" as "[A B]". iFrame. iSplits; ss; et. } *)
+    (* } *)
+    (* econs; ss. *)
+    (* { init. harg. mDesAll. des; clarify. unfold runF, ccallU. steps. *)
+    (*   mDesOr "INV"; mDesAll; des; clarify. *)
+    (*   1: { mAssertPure False; ss. iCombine "INV A" as "A". iOwnWf "A" as WF0. admit "ez". } *)
+    (*   steps. rewrite Any.upcast_downcast in *. clarify. steps. *)
+    (*   hcall _ _ _ with "INV"; auto. *)
+    (*   { esplits; ss. } *)
+    (*   steps. mDesAll; clarify. mDesOr "INV1"; mDesAll; clarify. *)
+    (*   1: { mAssertPure False; ss. iCombine "INV1 A" as "A". iOwnWf "A" as WF0. admit "ez". } *)
+    (*   rewrite _UNWRAPU. steps. *)
+    (*   hret _; ss. *)
+    (*   { iFrame. iSplits; ss; et. } *)
+    (* } *)
+  Unshelve. all: ss. all: try exact 0.
+  Qed.
+
+End SIMMODSEM.
